src/Std/Internal/Do/Triple/Gadget.lean
@@ -7,7 +7,7 @@ module
 
 prelude
 public import Std.Internal.Do.Triple.Basic
-public import Std.Internal.Do.Order.Heyting
+public import Std.Internal.Order.Heyting
 
 @[expose] public section
 
